Update CompCertO
The semantics of categorical composition and flat composition has been
simplified by dropping the footprint related conditions in transitions. On the
other hand, we put restrictions on the programs being composed to rule out the
situations where those footprint related conditions used to come into play.

compcertox/Lifting.v
@@ -7,7 +7,6 @@ Require Import CategoricalComp.
 Require Import SmallstepLinking_.
 Require Import Smallstep_.
 Require Import Linking.
-Require Import CompCertO.
 
 (* Definitions *)
 Section Lifting.
@@ -30,18 +29,13 @@ Section Lifting.
   Program Definition lifted_lts: lts liAX liBX stateX :=
     {|
       genvtype := genvtype L;
-      step p ge '(s, a) t '(s', a') := (step L p ge s t s' /\ a = a')%type;
+      step ge '(s, a) t '(s', a') := (step L ge s t s' /\ a = a')%type;
       initial_state := (initial_state L) * eq;
       at_external := fun s (q: query liAX) => ((at_external L) * eq) s q;
       after_external s := (after_external L (fst s)) * eq;
       final_state := (final_state L) * eq;
       globalenv := globalenv L
     |}%rel.
-  Next Obligation.
-    destruct s, s'. split.
-    eapply steps_monotone; now eauto.
-    easy.
-  Qed.
 
 End Lifting.
 
@@ -86,7 +80,7 @@ Section CAT_COMP_LIFT.
     (comp_semantics' L1 L2 sk) @ K ≤ comp_semantics' (L1 @ K) (L2 @ K) sk.
   Proof.
     constructor. econstructor. reflexivity. intros i. reflexivity.
-    intros se _ [ ] ? [ ] Hse. instantiate (1 := fun _ _ _ => _). cbn beta.
+    intros se _ [ ] [ ] Hse. instantiate (1 := fun _ _ _ => _). cbn beta.
     eapply forward_simulation_step with (match_states := state_match).
     - intros q _ s1 [ ] Hq. destruct s1 as [s1 ks].
       inv Hq. inv H. destruct q as [q k]. cbn in *. subst.
@@ -99,7 +93,7 @@ Section CAT_COMP_LIFT.
       inv Hq. inv H. cbn in *. subst. inv Hs. constructor; auto.
       constructor; auto.
       intros [r1 kr1] [r2 kr2] [s1' k1'] [ ] Hr. inv Hr. inv H.
-      inv Hq. inv H. cbn in *. subst. inv Hs. inv H8.
+      inv Hq. inv H. cbn in *. subst. inv Hs. inv H6.
       eexists; split; repeat econstructor; eauto.
     - intros [s1 k1] t [s1' k1'] Hstep s2 Hs.
       inv Hstep. inv H; inv Hs.
@@ -124,7 +118,7 @@ Section CAT_COMP_LIFT.
     comp_semantics' (L1 @ K) (L2 @ K) sk ≤ (comp_semantics' L1 L2 sk) @ K.
   Proof.
     constructor. econstructor. reflexivity. intros i. reflexivity.
-    intros se _ [ ] ? [ ] Hse. instantiate (1 := fun _ _ _ => _). cbn beta.
+    intros se _ [ ] [ ] Hse. instantiate (1 := fun _ _ _ => _). cbn beta.
     eapply forward_simulation_step
       with (match_states := fun s1 s2 => state_match s2 s1).
     - intros [q1 kq] _ s [ ] H. inv H. inv H0.
@@ -133,11 +127,11 @@ Section CAT_COMP_LIFT.
     - intros s1 [s2 ks] [r kr] Hs H. inv H. inv H0.
       destruct s. cbn in *. subst. inv Hs.
       eexists (_, _). split; repeat (cbn; econstructor); auto.
-    - intros s1 [s2 ks] [q kq] Hs H. inv H. inv H2.
+    - intros s1 [s2 ks] [q kq] Hs H. inv H. inv H0.
       cbn in *. subst. inv Hs. cbn in *.
-      eexists _, (_, _).
+      eexists tt, (_, _).
       repeat apply conj; repeat constructor; eauto.
-      intros [r1 kr1] [r2 kr2] s1' <- Hr. inv Hr. inv H6.
+      intros [r1 kr1] [r2 kr2] s1' <- Hr. inv Hr. inv H4.
       destruct s2'. cbn in *. subst.
       eexists; split; repeat (cbn; econstructor); eauto.
       cbn. constructor; auto.
@@ -156,7 +150,6 @@ Section CAT_COMP_LIFT.
         eexists (_, _); split; constructor; auto.
         eapply CategoricalComp.step_pop; eauto.
     - apply well_founded_ltof.
-      Unshelve. exact tt.
   Qed.
 
   Lemma lift_categorical_comp:
@@ -185,7 +178,7 @@ Section HCOMP_LIFT.
   Proof.
     constructor. econstructor. reflexivity.
     intros i. reflexivity.
-    intros se _ [ ] ? [ ] Hse. instantiate (1 := fun _ _ _ => _). cbn beta.
+    intros se _ [ ] [ ] Hse. instantiate (1 := fun _ _ _ => _). cbn beta.
     eapply forward_simulation_step with (match_states := state_match_hcomp).
     - intros [q kq] ? [s ks] [ ] H. inv H. cbn in *. subst.
       inv H0. eexists. split.
@@ -228,7 +221,7 @@ Section HCOMP_LIFT.
   Proof.
     constructor. econstructor. reflexivity.
     intros i. reflexivity.
-    intros se _ [ ] ? [ ] Hse. instantiate (1 := fun _ _ _ => _). cbn beta.
+    intros se _ [ ] [ ] Hse. instantiate (1 := fun _ _ _ => _). cbn beta.
     eapply forward_simulation_step
       with (match_states := fun s1 s2 => state_match_hcomp s2 s1).
     - intros [q1 kq1] [q2 kq2] s1 [ ] H. inv H. inv H1.
@@ -277,17 +270,17 @@ Section HCOMP_LIFT.
 
 End HCOMP_LIFT.
 
-Lemma lifting_step_star {liA liB K} (L: Smallstep_.semantics liA liB) se qset s1 t s2 k:
-  Star (L se) qset s1 t s2 ->
-  Star(lifted_lts K (L se)) qset (s1, k) t (s2, k).
+Lemma lifting_step_star {liA liB K} (L: Smallstep_.semantics liA liB) se s1 t s2 k:
+  Star (L se) s1 t s2 ->
+  Star(lifted_lts K (L se)) (s1, k) t (s2, k).
 Proof.
   induction 1; [eapply star_refl | eapply star_step]; eauto.
   constructor; auto.
 Qed.
 
-Lemma lifting_step_plus {liA liB K} (L: Smallstep_.semantics liA liB) se qset s1 t s2 k:
-  Plus (L se) qset s1 t s2 ->
-  Plus (lifted_lts K (L se)) qset (s1, k) t (s2, k).
+Lemma lifting_step_plus {liA liB K} (L: Smallstep_.semantics liA liB) se s1 t s2 k:
+  Plus (L se) s1 t s2 ->
+  Plus (lifted_lts K (L se)) (s1, k) t (s2, k).
 Proof.
   destruct 1; econstructor; eauto using lifting_step_star.
   split; eauto.
@@ -304,8 +297,8 @@ Proof.
   - apply (fsim_skel H).
   - intros i. apply (fsim_footprint H).
   - destruct H as [? ? ? ? ? Hf ?]. cbn. clear -Hf.
-    intros se1 se2 [ ] qset Hse Hse'.
-    specialize (Hf se1 se2 tt qset Hse Hse'). subst.
+    intros se1 se2 [ ] Hse Hse'.
+    specialize (Hf se1 se2 tt Hse Hse'). subst.
     econstructor.
     + intros [q kq] ? [s1 ks] [ ] Hi. inv Hi. cbn in *; subst.
       exploit (fsim_match_initial_states Hf); eauto. econstructor.
@@ -337,9 +330,9 @@ Qed.
 
 Definition skel_extend {liA liB} (L: Smallstep_.semantics liA liB) sk :=
   {|
-  activate se := L se;
-  skel := sk;
-  footprint := footprint L;
+    activate se := L se;
+    skel := sk;
+    footprint := footprint L;
   |}.
 
 (* Lifting a code skeleton *)
