compcertox/Composition.v
@@ -5,7 +5,7 @@ Require Import CallconvAlgebra_.
 Require Import LanguageInterface_ Events Globalenvs Smallstep_ CategoricalComp FlatComp.
 Require Import Memory Values.
 Require Import Clight_ Linking.
-Require Import AbstractStateRel Lifting CModule CompCertO.
+Require Import AbstractStateRel Lifting CModule.
 
 Definition layer_comp {K} (M: cmodule) (L: layer K) sk :=
   comp_semantics' (semantics M sk @ K) L sk.
@@ -46,7 +46,7 @@ Section SKEL_EXT.
   Proof.
     constructor. eapply Forward_simulation with _ (fun _ _ _ => _); auto.
     - intros. reflexivity.
-    - intros se ? [ ] qset [ ] Hse.
+    - intros se ? [ ] [ ] Hse.
       eapply forward_simulation_plus with (match_states := eq);
         cbn; intros; subst; eauto 10 using plus_one.
       exists tt, q1. intuition (subst; eauto).
@@ -59,6 +59,8 @@ Section VCOMP.
   Context {K1 K2 K3 L1 L2 L3} {M N: cmodule}
           {R: rel_adt K1 K2} {S: rel_adt K2 K3}
           (HL1: ksim L1 L2 M R) (HL2: ksim L2 L3 N S).
+  (* FIXME: the linkable hypothesis should be simplified *)
+  Context `{!CategoricalLinkable (semantics M (skel L1)) (semantics N (skel L1))}.
 
   Theorem layer_vcomp: ksim L1 L3 (M ++ N) (R ∘ S).
   Proof.
@@ -105,20 +107,32 @@ Section VCOMP.
 
 End VCOMP.
 
-(* Section HCOMP. *)
+Section HCOMP.
 
-(*   Context {K1 K2 L1 L2 L3} {M N: cmodule} {R: rel_adt K1 K2} *)
-(*           (HL1: ksim L1 L3 M R) (HL2: ksim L2 L3 N R). *)
+  Generalizable All Variables.
+  Context `{R: rel_adt K1 K2}
+          {M N: cmodule} `(HL1: ksim L1 L3 M R) `(HL2: ksim L2 L3 N R).
+  Variable (sk: AST.program unit unit).
+  Hypothesis (Hk1: linkorder (skel L1) sk)
+             (Hk2: linkorder (skel L2) sk).
+  (* Theorem layer_hcomp L: *)
+  (*   L1 ⊎ L2 = Some L -> ksim L L3 (M ⊕ N) R. *)
+  (* Admitted. *)
 
-(*   Theorem layer_hcomp L: *)
-(*     L1 ⊎ L2 = Some L -> ksim L L3 (M ⊕ N) R. *)
-(*   Admitted. *)
+  (* Naming convention: *)
+  (*      xxx is the composition definition or lemma with linked skeleton *)
+  (*      xxx' is the same with a provided code skeleton *)
+  Theorem layer_hcomp':
+    ksim (flat_comp_semantics' L1 L2 sk) L3 (M ++ N) R.
+  Proof.
+    unfold ksim in *.
+    destruct HL1 as [Hsk1 [Hmod1 H1]]. clear HL1.
+    destruct HL2 as [Hsk2 [Hmod2 H2]]. clear HL2.
+    split. eapply linkorder_trans; eauto.
+    split. apply compatible_app; (eapply compatible_trans; [ | eauto]); eauto.
 
-(*   (* Naming convention: *)
-(*      xxx is the composition definition or lemma with linked skeleton *)
-(*      xxx' is the same with a provided code skeleton *) *)
-(*   Theorem layer_hcomp' sk: *)
-(*     ksim (flat_comp_semantics' L1 L2 sk) L3 (M ⊕ N) R. *)
-(*   Admitted. *)
 
-(* End HCOMP. *)
+
+  Admitted.
+
+End HCOMP.
